Added state to Checkpoint messages.
Currently we use the map containing the CommittedClientOperations as
the state that we will transfer and verify. Later in the model development
we will have an additional set - ExecutedClientOperations that will be used
instead. We are keeping this change for the future to keep the model simple
for the first version of the proof and build up incrementally.
Also added a PerformStateTransfer step that slides the Working Window
further than the Working Window size.

docs/sbft-formal-model/proof.dfy
@@ -762,12 +762,34 @@ module Proof {
     && var h_v' := v'.hosts[step.id].replicaVariables;
     && Replica.NextStep(h_c, h_v, h_v', step.msgOps, h_step)
     && h_step.AdvanceWorkingWindowStep?
-    && Replica.AdvanceWorkingWindow(h_c, h_v, h_v', step.msgOps, h_step.seqID)
+    && Replica.AdvanceWorkingWindow(h_c, h_v, h_v', step.msgOps, h_step.seqID, h_step.checkpointsQuorum)
   }
 
   lemma AdvanceWorkingWindowStepPreservesInv(c: Constants, v:Variables, v':Variables, 
                                   step:Step, h_step:Replica.Step)
     requires AdvanceWorkingWindowStepIsEnabled(c, v, v', step, h_step)
+    ensures Inv(c, v')
+  {
+    CommitMsgStability(c, v, v', step);
+  }
+
+  predicate PerformStateTransferStepIsEnabled(c: Constants, v:Variables, v':Variables,
+                                   step:Step, h_step:Replica.Step)
+  {
+    && Inv(c, v)
+    && NextStep(c, v, v', step)
+    && IsHonestReplica(c, step.id)
+    && var h_c := c.hosts[step.id].replicaConstants;
+    && var h_v := v.hosts[step.id].replicaVariables;
+    && var h_v' := v'.hosts[step.id].replicaVariables;
+    && Replica.NextStep(h_c, h_v, h_v', step.msgOps, h_step)
+    && h_step.PerformStateTransferStep?
+    && Replica.PerformStateTransfer(h_c, h_v, h_v', step.msgOps, h_step.seqID, h_step.checkpointsQuorum)
+  }
+
+  lemma PerformStateTransferStepPreservesInv(c: Constants, v:Variables, v':Variables, 
+                                  step:Step, h_step:Replica.Step)
+    requires PerformStateTransferStepIsEnabled(c, v, v', step, h_step)
     ensures Inv(c, v')
   {
     CommitMsgStability(c, v, v', step);
@@ -952,8 +974,11 @@ module Proof {
         case RecvCheckpointStep() => {
           RecvCheckpointStepPreservesInv(c, v, v', step, h_step);
         }
-        case AdvanceWorkingWindowStep(seqID) => {
+        case AdvanceWorkingWindowStep(seqID, checkpointsQuorum) => {
           AdvanceWorkingWindowStepPreservesInv(c, v, v', step, h_step);
+        }
+        case PerformStateTransferStep(seqID, checkpointsQuorum) => {
+          PerformStateTransferStepPreservesInv(c, v, v', step, h_step);
         }
         case LeaveViewStep(newView) => {
           LeaveViewStepPreservesInv(c, v, v', step, h_step);
